\documentclass[../main.tex]{subfiles}
\begin{document}
\subsection{The adjoint equation}\label{subsec3.1}
Consider the SDE \cite[Sub-section 4.3.1, p.93]{Gardiner03}
\begin{equation*}
        dx = f(x,t)dt + \sqrt{g(x,t)}dW\,,
\end{equation*}
then the FPE \cite[Sub-section 4.3.4, p.96]{Gardiner03} reads
\begin{equation*}
     \partial_{t}p(x,t|y,0) = -\partial_{x}\big(f(x,t)p(x,t|y,0)\big)+\frac{1}{2}\partial_{xx}^{2}\big(g(x,t)p(x,t|y,0)\big)\,.
\end{equation*}
The adjoint FPE \cite[Section 3.6, p.55]{Gardiner03} reads
\begin{equation*}
     \partial_{t}p(x,0|y,t) = -f(y,t)\partial_{y}p(x,0|y,t)-\frac{1}{2}g(y,t)\partial_{yy}^{2}p(x,0|y,t)\,.
\end{equation*}
If both $f$ and $g$ are time-independent then the solution $x(t)$ is said to be \textit{homogeneous} \cite[Section 3.7, p.56]{Gardiner03} and as such its conditional transition probability is
\begin{equation*}
     p(x,t|y,0) = p(x,0|y,-t)\,,
\end{equation*}
\begin{equation*}
     \partial_{t}p(x,t|y,0)=\partial_{t}p(x,0|y,-t)=-\partial_{(-t)}p(x,0|y,-t)\,,
\end{equation*}
where the last equality is guaranteed by the chain-rule
\begin{equation*}
     g(x)=-x\,,\quad \big(f\circ g\big)(x) = g\big(f(x)\big) = -f(x)\,.
\end{equation*}
\begin{equation*}
     \frac{dg}{dx} = \frac{dg}{df}\frac{df}{dx} = -\frac{df}{dx}\,.
\end{equation*}
It follows immediately that the adjoint FPE can be rewritten as 
\begin{align*}
        \partial_{t}p(x,0|y,t) &= -\partial_{(-t)}p(x,0|y,-t) = -\Big(-f(y)\partial_{y}p(x,0|y,-t)-\frac{1}{2}g(y)\partial_{yy}^{2}p(x,0|y,-t)\Big) = \nonumber \\ 
                                     &=  f(y)\partial_{y}p(x,0|y,-t)+\frac{1}{2}g(y)\partial_{yy}^{2}p(x,0|y,-t) = \nonumber \\
                                     &=  f(y)\partial_{y}p(x,t|y,0)+\frac{1}{2}g(y)\partial_{yy}^{2}p(x,t|y,0) = \nonumber \\
                                     &= -\partial_{t}p(x,t|y,0) \,.
\end{align*}
\end{document}
